Rename to more traditional program logic names

prog/vfmLogicScript.sml
@@ -3,115 +3,115 @@ open HolKernel boolLib bossLib Parse
 
 val () = new_theory "vfmLogic";
 
-Definition valid_def:
-  valid P f Q =
+Definition spec_def:
+  spec P f Q =
   ∀s: execution_state.
     P s ⇒ case f s : α execution_result
           of (r, t) => Q r t
 End
 
-Definition valid_result_def:
-  valid_result P f Q =
-  valid P f (λr s. ISL r ∧ Q (OUTL r) s)
+Definition spec_total_def:
+  spec_total P f Q =
+  spec P f (λr s. ISL r ∧ Q (OUTL r) s)
 End
 
-Definition valid_result_fn_def:
-  valid_result_fn P f Q g =
-  valid_result P f (λr s. Q s ∧ r = g s)
+Definition spec_total_fn_def:
+  spec_total_fn P f Q g =
+  spec_total P f (λr s. Q s ∧ r = g s)
 End
 
-Definition valid_result_eq_def:
-  valid_result_eq P f Q x =
-  valid_result_fn P f Q (K x)
+Definition spec_total_eq_def:
+  spec_total_eq P f Q x =
+  spec_total_fn P f Q (K x)
 End
 
-Theorem valid_strengthen:
-  valid P f Q1 ∧
+Theorem spec_strengthen:
+  spec P f Q1 ∧
   (∀r s. Q1 r s ⇒ Q r s)
   ⇒
-  valid P f Q
+  spec P f Q
 Proof
-  rw[valid_def]
+  rw[spec_def]
   \\ last_x_assum drule \\ gvs[]
   \\ CASE_TAC \\ rw[]
 QED
 
-Theorem valid_weaken:
-  valid P1 f1 Q ∧ (∀s. P s ⇒ P1 s ∧ f1 = f) ⇒
-  valid P f Q
+Theorem spec_weaken:
+  spec P1 f1 Q ∧ (∀s. P s ⇒ P1 s ∧ f1 = f) ⇒
+  spec P f Q
 Proof
-  rw[valid_def]
+  rw[spec_def]
   \\ first_x_assum drule \\ rw[]
   \\ first_x_assum drule \\ rw[]
 QED
 
-Theorem valid_result_weaken:
-  valid_result P1 f1 Q ∧ (∀s. P s ⇒ P1 s ∧ f1 = f) ⇒
-  valid_result P f Q
+Theorem spec_total_weaken:
+  spec_total P1 f1 Q ∧ (∀s. P s ⇒ P1 s ∧ f1 = f) ⇒
+  spec_total P f Q
 Proof
-  rw[valid_result_def]
-  \\ metis_tac[valid_weaken]
+  rw[spec_total_def]
+  \\ metis_tac[spec_weaken]
 QED
 
-Theorem valid_result_fn_weaken:
-  valid_result_fn P1 f1 Q g ∧ (∀s. P s ⇒ P1 s ∧ f1 = f) ⇒
-  valid_result_fn P f Q g
+Theorem spec_total_fn_weaken:
+  spec_total_fn P1 f1 Q g ∧ (∀s. P s ⇒ P1 s ∧ f1 = f) ⇒
+  spec_total_fn P f Q g
 Proof
-  rw[valid_result_fn_def]
-  \\ metis_tac[valid_result_weaken]
+  rw[spec_total_fn_def]
+  \\ metis_tac[spec_total_weaken]
 QED
 
-Theorem valid_result_eq_weaken:
-  valid_result_eq P1 f1 Q g ∧ (∀s. P s ⇒ P1 s ∧ f1 = f) ⇒
-  valid_result_eq P f Q g
+Theorem spec_total_eq_weaken:
+  spec_total_eq P1 f1 Q g ∧ (∀s. P s ⇒ P1 s ∧ f1 = f) ⇒
+  spec_total_eq P f Q g
 Proof
-  rw[valid_result_eq_def]
-  \\ metis_tac[valid_result_fn_weaken]
+  rw[spec_total_eq_def]
+  \\ metis_tac[spec_total_fn_weaken]
 QED
 
-Theorem valid_result_valid:
-  valid_result P f Q1 ∧
+Theorem spec_total_spec:
+  spec_total P f Q1 ∧
   (∀r s. ISL r ∧ Q1 (OUTL r) s ⇒ Q r s)
   ⇒
-  valid P f Q
+  spec P f Q
 Proof
-  rw[valid_result_def]
-  \\ irule valid_strengthen
+  rw[spec_total_def]
+  \\ irule spec_strengthen
   \\ goal_assum (first_x_assum o mp_then Any mp_tac)
   \\ rw[]
 QED
 
-Theorem valid_result_eq_valid_result:
-  valid_result_eq P f Q1 x ∧
+Theorem spec_total_eq_spec_total:
+  spec_total_eq P f Q1 x ∧
   (∀s. Q1 s ⇒ Q x s)
   ⇒
-  valid_result P f Q
+  spec_total P f Q
 Proof
-  rw[valid_result_fn_def, valid_result_eq_def, valid_result_def]
-  \\ irule valid_strengthen
+  rw[spec_total_fn_def, spec_total_eq_def, spec_total_def]
+  \\ irule spec_strengthen
   \\ goal_assum (first_x_assum o mp_then Any mp_tac)
   \\ rw[]
 QED
 
-Theorem valid_bind:
-  valid_result P g Q1 ∧
-  (∀x. valid (Q1 x) (f x) Q)
+Theorem spec_bind:
+  spec_total P g Q1 ∧
+  (∀x. spec (Q1 x) (f x) Q)
   ⇒
-  valid P (monad_bind g f) Q
+  spec P (monad_bind g f) Q
 Proof
-  rw[valid_result_def, valid_def, bind_def]
+  rw[spec_total_def, spec_def, bind_def]
   \\ CASE_TAC \\ gvs[]
   \\ last_x_assum drule \\ rw[]
   \\ CASE_TAC \\ gvs[]
 QED
 
-Theorem valid_ignore_bind:
-  valid_result P r Q1 ∧
-  (∀x. valid (Q1 x) f Q)
+Theorem spec_ignore_bind:
+  spec_total P r Q1 ∧
+  (∀x. spec (Q1 x) f Q)
   ⇒
-  valid P (ignore_bind r f) Q
+  spec P (ignore_bind r f) Q
 Proof
-  rw[valid_def, valid_result_def, ignore_bind_def, bind_def]
+  rw[spec_def, spec_total_def, ignore_bind_def, bind_def]
   \\ first_x_assum drule
   \\ CASE_TAC \\ gvs[] \\ strip_tac
   \\ CASE_TAC \\ gvs[]
@@ -119,132 +119,132 @@ Proof
   \\ first_x_assum drule \\ rw[]
 QED
 
-Theorem valid_result_bind:
-  valid_result P g Q1 ∧
-  (∀x. valid_result (Q1 x) (f x) Q)
+Theorem spec_total_bind:
+  spec_total P g Q1 ∧
+  (∀x. spec_total (Q1 x) (f x) Q)
   ⇒
-  valid_result P (monad_bind g f) Q
+  spec_total P (monad_bind g f) Q
 Proof
   rw[]
-  \\ rw[valid_result_def]
-  \\ irule valid_bind
+  \\ rw[spec_total_def]
+  \\ irule spec_bind
   \\ goal_assum(first_assum o mp_then Any mp_tac)
   \\ rw[]
-  \\ irule valid_result_valid
+  \\ irule spec_total_spec
   \\ qexists_tac`Q` \\ rw[]
 QED
 
-Theorem valid_result_ignore_bind:
-  valid_result P r Q1 ∧
-  (∀x. valid_result (Q1 x) f Q)
+Theorem spec_total_ignore_bind:
+  spec_total P r Q1 ∧
+  (∀x. spec_total (Q1 x) f Q)
   ⇒
-  valid_result P (ignore_bind r f) Q
+  spec_total P (ignore_bind r f) Q
 Proof
   rw[]
-  \\ rw[valid_result_def]
-  \\ irule valid_ignore_bind
+  \\ rw[spec_total_def]
+  \\ irule spec_ignore_bind
   \\ goal_assum(first_assum o mp_then Any mp_tac)
   \\ rw[]
-  \\ irule valid_result_valid
+  \\ irule spec_total_spec
   \\ qexists_tac`Q` \\ rw[]
 QED
 
-Theorem valid_result_fn_bind:
-  valid_result P g Q1 ∧
-  (∀x. valid_result_fn (Q1 x) (f x) Q h)
+Theorem spec_total_fn_bind:
+  spec_total P g Q1 ∧
+  (∀x. spec_total_fn (Q1 x) (f x) Q h)
   ⇒
-  valid_result_fn P (monad_bind g f) Q h
+  spec_total_fn P (monad_bind g f) Q h
 Proof
   rw[]
-  \\ rw[valid_result_fn_def]
-  \\ irule valid_result_bind
+  \\ rw[spec_total_fn_def]
+  \\ irule spec_total_bind
   \\ goal_assum(first_assum o mp_then Any mp_tac)
   \\ rw[]
-  \\ fs[valid_result_fn_def]
+  \\ fs[spec_total_fn_def]
 QED
 
-Theorem valid_result_eq_bind:
-  valid_result P g Q1 ∧
-  (∀x. valid_result_eq (Q1 x) (f x) Q y)
+Theorem spec_total_eq_bind:
+  spec_total P g Q1 ∧
+  (∀x. spec_total_eq (Q1 x) (f x) Q y)
   ⇒
-  valid_result_eq P (monad_bind g f) Q y
+  spec_total_eq P (monad_bind g f) Q y
 Proof
-  rw[valid_result_eq_def]
-  \\ irule valid_result_fn_bind
+  rw[spec_total_eq_def]
+  \\ irule spec_total_fn_bind
   \\ goal_assum(first_assum o mp_then Any mp_tac)
   \\ rw[]
 QED
 
-Theorem valid_result_fn_ignore_bind:
-  valid_result P g Q1 ∧
-  (∀x. valid_result_fn (Q1 x) f Q h)
+Theorem spec_total_fn_ignore_bind:
+  spec_total P g Q1 ∧
+  (∀x. spec_total_fn (Q1 x) f Q h)
   ⇒
-  valid_result_fn P (ignore_bind g f) Q h
+  spec_total_fn P (ignore_bind g f) Q h
 Proof
   rw[]
-  \\ rw[valid_result_fn_def]
-  \\ irule valid_result_ignore_bind
+  \\ rw[spec_total_fn_def]
+  \\ irule spec_total_ignore_bind
   \\ goal_assum(first_assum o mp_then Any mp_tac)
   \\ rw[]
-  \\ fs[valid_result_fn_def]
+  \\ fs[spec_total_fn_def]
 QED
 
-Theorem valid_result_eq_ignore_bind:
-  valid_result P g Q1 ∧
-  (∀x. valid_result_eq (Q1 x) f Q y)
+Theorem spec_total_eq_ignore_bind:
+  spec_total P g Q1 ∧
+  (∀x. spec_total_eq (Q1 x) f Q y)
   ⇒
-  valid_result_eq P (ignore_bind g f) Q y
+  spec_total_eq P (ignore_bind g f) Q y
 Proof
-  rw[valid_result_eq_def]
-  \\ irule valid_result_fn_ignore_bind
+  rw[spec_total_eq_def]
+  \\ irule spec_total_fn_ignore_bind
   \\ goal_assum(first_assum o mp_then Any mp_tac)
   \\ rw[]
 QED
 
-Theorem valid_result_eq_eq_ignore_bind:
-  valid_result_eq P g Q1 z ∧
-  valid_result_eq Q1 f Q y
+Theorem spec_total_eq_eq_ignore_bind:
+  spec_total_eq P g Q1 z ∧
+  spec_total_eq Q1 f Q y
   ⇒
-  valid_result_eq P (ignore_bind g f) Q y
+  spec_total_eq P (ignore_bind g f) Q y
 Proof
-  rw[valid_result_eq_def]
-  \\ irule valid_result_fn_ignore_bind
-  \\ gs[valid_result_fn_def]
+  rw[spec_total_eq_def]
+  \\ irule spec_total_fn_ignore_bind
+  \\ gs[spec_total_fn_def]
   \\ goal_assum(first_assum o mp_then Any mp_tac)
   \\ rw[]
-  \\ irule valid_result_weaken
+  \\ irule spec_total_weaken
   \\ goal_assum(first_assum o mp_then Any mp_tac)
   \\ rw[]
 QED
 
-Theorem valid_result_get_current_context:
+Theorem spec_total_get_current_context:
   (∀s. P s ⇒ ¬NULL s.contexts) ∧
   (∀s. P s ⇒ Q (HD s.contexts) s)
   ⇒
-  valid_result P get_current_context Q
+  spec_total P get_current_context Q
 Proof
-  rw[valid_result_def, valid_def, get_current_context_def]
+  rw[spec_total_def, spec_def, get_current_context_def]
   \\ rw[fail_def, return_def]
   \\ rpt(first_x_assum drule)
   \\ rw[]
 QED
 
-Theorem valid_result_eq_assert:
+Theorem spec_total_eq_assert:
   (∀s. P s ⇒ b ∧ Q s)
   ⇒
-  valid_result_eq P (assert b e) Q ()
+  spec_total_eq P (assert b e) Q ()
 Proof
-  rw[valid_result_eq_def, valid_result_fn_def, valid_result_def, valid_def, assert_def]
+  rw[spec_total_eq_def, spec_total_fn_def, spec_total_def, spec_def, assert_def]
 QED
 
-Theorem valid_result_eq_set_current_context:
+Theorem spec_total_eq_set_current_context:
   (∀s. P s ⇒ ¬NULL s.contexts) ∧
   (∀s. P s ⇒ Q (s with contexts updated_by λls. c :: TL ls))
   ⇒
-  valid_result_eq P (set_current_context c) Q ()
+  spec_total_eq P (set_current_context c) Q ()
 Proof
-  rw[valid_result_eq_def, valid_result_def, valid_def,
-     valid_result_fn_def, set_current_context_def]
+  rw[spec_total_eq_def, spec_total_def, spec_def,
+     spec_total_fn_def, set_current_context_def]
   \\ last_x_assum drule \\ rw[return_def]
   \\ last_x_assum drule \\ rw[]
   \\ qmatch_goalsub_abbrev_tac`Q s1`
@@ -253,32 +253,32 @@ Proof
   \\ rw[]
 QED
 
-Theorem valid_result_handle:
-  valid_result P f Q
+Theorem spec_total_handle:
+  spec_total P f Q
   ⇒
-  valid_result P (handle f g) Q
+  spec_total P (handle f g) Q
 Proof
-  rw[valid_result_def, valid_def, handle_def]
+  rw[spec_total_def, spec_def, handle_def]
   \\ first_x_assum drule
   \\ CASE_TAC \\ rw[]
   \\ CASE_TAC \\ rw[]
   \\ gvs[]
 QED
 
-Theorem valid_result_fn_handle:
-  valid_result_fn P f Q k
+Theorem spec_total_fn_handle:
+  spec_total_fn P f Q k
   ⇒
-  valid_result_fn P (handle f g) Q k
+  spec_total_fn P (handle f g) Q k
 Proof
-  rw[valid_result_fn_def, valid_result_handle]
+  rw[spec_total_fn_def, spec_total_handle]
 QED
 
-Theorem valid_result_eq_handle:
-  valid_result_eq P f Q ()
+Theorem spec_total_eq_handle:
+  spec_total_eq P f Q ()
   ⇒
-  valid_result_eq P (handle f g) Q ()
+  spec_total_eq P (handle f g) Q ()
 Proof
-  rw[valid_result_eq_def, valid_result_fn_handle]
+  rw[spec_total_eq_def, spec_total_fn_handle]
 QED
 
 Definition has_cc_def:
@@ -297,30 +297,30 @@ Proof
   rw[] \\ rw[]
 QED
 
-Theorem valid_result_eq_consume_gas:
+Theorem spec_total_eq_consume_gas:
   (∀s. P s ⇒ has_cc (λc. c.gasUsed + n ≤ c.msgParams.gasLimit) s) ∧
   (∀s. P s ⇒ Q (update_cc (λc. c with gasUsed updated_by $+ n) s))
   ⇒
-  valid_result_eq P (consume_gas n) Q ()
+  spec_total_eq P (consume_gas n) Q ()
 Proof
   rw[consume_gas_def]
-  \\ irule valid_result_eq_bind
+  \\ irule spec_total_eq_bind
   \\ qexists_tac`λr s. P s ∧ r = HD s.contexts`
   \\ reverse(rw[])
   >- (
-    irule valid_result_get_current_context
+    irule spec_total_get_current_context
     \\ rw[] \\ res_tac \\ fs[has_cc_def])
-  \\ irule valid_result_eq_ignore_bind
+  \\ irule spec_total_eq_ignore_bind
   \\ qexists_tac`λr s. P s ∧ x = HD s.contexts`
   \\ reverse(rw[])
   >- (
-    irule valid_result_eq_valid_result \\ rw[]
+    irule spec_total_eq_spec_total \\ rw[]
     \\ qexists_tac`λs. P s ∧ x = HD s.contexts` \\ rw[]
-    \\ irule valid_result_eq_assert
+    \\ irule spec_total_eq_assert
     \\ rw[]
     \\ last_x_assum drule \\ rw[has_cc_def]
     \\ rw[] )
-  \\ irule valid_result_eq_set_current_context
+  \\ irule spec_total_eq_set_current_context
   \\ rw[]
   \\ last_x_assum drule \\ rw[has_cc_def]
   \\ last_x_assum drule \\ rw[]
@@ -329,33 +329,33 @@ Proof
         context_component_equality, update_cc_def]
 QED
 
-Theorem valid_result_eq_push_stack:
+Theorem spec_total_eq_push_stack:
   (∀s. P s ⇒ has_cc (λc. LENGTH c.stack < stack_limit) s) ∧
   (∀s. P s ⇒ Q (update_cc (λc. c with stack updated_by CONS w) s))
   ⇒
-  valid_result_eq P (push_stack w) Q ()
+  spec_total_eq P (push_stack w) Q ()
 Proof
   (* TODO: mostly repeated from previous proof - abstract or automate? *)
   rw[push_stack_def]
-  \\ irule valid_result_eq_bind \\ rw[]
+  \\ irule spec_total_eq_bind \\ rw[]
   \\ qexists_tac`λr s. P s ∧ r = HD s.contexts`
   \\ reverse(rw[])
   >- (
-    irule valid_result_get_current_context
+    irule spec_total_get_current_context
     \\ rw[]
     \\ last_x_assum drule \\ rw[has_cc_def]
     \\ rw[] )
-  \\ irule valid_result_eq_ignore_bind \\ rw[]
+  \\ irule spec_total_eq_ignore_bind \\ rw[]
   \\ qexists_tac`λr s. P s ∧ x = HD s.contexts`
   \\ reverse(rw[])
   >- (
-    irule valid_result_eq_valid_result \\ rw[]
+    irule spec_total_eq_spec_total \\ rw[]
     \\ qexists_tac`λs. P s ∧ x = HD s.contexts` \\ rw[]
-    \\ irule valid_result_eq_assert
+    \\ irule spec_total_eq_assert
     \\ rw[]
     \\ last_x_assum drule \\ rw[has_cc_def]
     \\ rw[] )
-  \\ irule valid_result_eq_set_current_context
+  \\ irule spec_total_eq_set_current_context
   \\ rw[]
   \\ last_x_assum drule \\ rw[has_cc_def]
   \\ last_x_assum drule \\ rw[]
@@ -364,7 +364,7 @@ Proof
         context_component_equality, update_cc_def]
 QED
 
-Theorem valid_result_eq_step_push:
+Theorem spec_total_eq_step_push:
   g = static_gas (Push n ws) ∧
   w = word_of_bytes F 0w (REVERSE ws) ∧
   (∀s. P s ⇒ has_cc (λc.
@@ -374,21 +374,21 @@ Theorem valid_result_eq_step_push:
                   stack updated_by CONS w
                 ; gasUsed updated_by $+ g |>) s))
   ⇒
-  valid_result_eq P (step_push n ws) Q ()
+  spec_total_eq P (step_push n ws) Q ()
 Proof
   rw[step_push_def, Excl"static_gas_def"]
   \\ qmatch_goalsub_abbrev_tac`consume_gas g`
   \\ qmatch_goalsub_abbrev_tac`push_stack w`
-  \\ irule valid_result_eq_ignore_bind \\ rw[]
+  \\ irule spec_total_eq_ignore_bind \\ rw[]
   \\ qexists_tac`λr s. has_cc (λc. LENGTH c.stack < stack_limit) s ∧
                        Q (update_cc (λc. c with stack updated_by CONS w) s)`
   \\ reverse (rw[])
   >- (
-    irule valid_result_eq_valid_result
+    irule spec_total_eq_spec_total
     \\ qmatch_goalsub_abbrev_tac`_ ⇒ Q1 _ _`
     \\ qexists_tac`λs. Q1 () s`
     \\ rw[Abbr`Q1`]
-    \\ irule valid_result_eq_consume_gas
+    \\ irule spec_total_eq_consume_gas
     \\ rw[]
     \\ last_x_assum drule \\ rw[has_cc_def]
     \\ rw[update_cc_def]
@@ -396,34 +396,34 @@ Proof
     \\ irule mp_rand \\ goal_assum drule
     \\ rw[execution_state_component_equality,
          context_component_equality, update_cc_def])
-  \\ irule valid_result_eq_push_stack
+  \\ irule spec_total_eq_push_stack
   \\ rw[]
 QED
 
-Theorem valid_result_eq_inc_pc_or_jump_inc:
+Theorem spec_total_eq_inc_pc_or_jump_inc:
   n = LENGTH (opcode i) ∧ ¬is_call i ∧
   (∀s. P s ⇒ has_cc (λc. c.jumpDest = NONE) s) ∧
   (∀s. P s ⇒ Q (update_cc (λc. c with pc updated_by $+ n) s))
   ⇒
-  valid_result_eq P (inc_pc_or_jump i) Q ()
+  spec_total_eq P (inc_pc_or_jump i) Q ()
 Proof
   rw[inc_pc_or_jump_def]
-  \\ irule valid_result_eq_bind
+  \\ irule spec_total_eq_bind
   \\ qexists_tac`λr s. P s ∧ r = HD s.contexts`
   \\ reverse conj_tac
   >- (
-    irule valid_result_get_current_context
+    irule spec_total_get_current_context
     \\ rw[]
     \\ last_x_assum drule \\ rw[has_cc_def]
     \\ rw[] )
   \\ rw[]
   \\ reverse(Cases_on`x.jumpDest`)
   >- (
-    rw[valid_result_eq_def, valid_result_fn_def, valid_result_def, valid_def]
+    rw[spec_total_eq_def, spec_total_fn_def, spec_total_def, spec_def]
     \\ last_x_assum drule \\ rw[has_cc_def]
     \\ gs[] )
   \\ rw[]
-  \\ irule valid_result_eq_set_current_context
+  \\ irule spec_total_eq_set_current_context
   \\ rw[]
   \\ last_x_assum drule \\ rw[has_cc_def]
   \\ last_x_assum drule \\ rw[]
@@ -432,36 +432,36 @@ Proof
         context_component_equality, update_cc_def]
 QED
 
-Theorem valid_result_eq_step:
+Theorem spec_total_eq_step:
   (∀s. P s ⇒ has_cc (λc.
     c.pc < LENGTH c.msgParams.code ∧
     FLOOKUP c.msgParams.parsed c.pc = SOME op) s) ∧
-  valid_result_eq P (do step_inst op; inc_pc_or_jump op od) Q ()
+  spec_total_eq P (do step_inst op; inc_pc_or_jump op od) Q ()
   ⇒
-  valid_result_eq P step Q ()
+  spec_total_eq P step Q ()
 Proof
   rw[step_def]
-  \\ irule valid_result_eq_handle
-  \\ irule valid_result_eq_bind \\ rw[]
+  \\ irule spec_total_eq_handle
+  \\ irule spec_total_eq_bind \\ rw[]
   \\ qexists_tac`λr s. P s ∧ r = HD s.contexts`
   \\ rw[]
   >- (
-    rw[valid_result_eq_def, valid_result_fn_def, valid_result_def, valid_def]
+    rw[spec_total_eq_def, spec_total_fn_def, spec_total_def, spec_def]
     \\ first_x_assum drule
     \\ rw[has_cc_def]
     \\ gvs[] )
   \\ TRY (
-    irule valid_result_get_current_context
+    irule spec_total_get_current_context
     \\ rw[]
     \\ first_x_assum drule
     \\ rw[has_cc_def]
     \\ rw[] )
   \\ CASE_TAC
   >- (
-    rw[valid_result_eq_def, valid_result_fn_def, valid_result_def, valid_def]
+    rw[spec_total_eq_def, spec_total_fn_def, spec_total_def, spec_def]
     \\ first_x_assum drule \\ rw[has_cc_def]
     \\ gvs[] )
-  \\ irule valid_result_eq_weaken
+  \\ irule spec_total_eq_weaken
   \\ goal_assum (first_assum o mp_then Any mp_tac)
   \\ rw[]
   \\ first_x_assum drule
@@ -469,33 +469,33 @@ Proof
   \\ gvs[]
 QED
 
-Theorem valid_imp:
-  valid P f Q ∧ P s
+Theorem spec_imp:
+  spec P f Q ∧ P s
   ⇒
   ∃r t. f s = (r, t) ∧ Q r t
 Proof
-  rw[valid_def]
+  rw[spec_def]
   \\ last_x_assum drule
   \\ CASE_TAC \\ rw[]
 QED
 
-Theorem valid_result_imp:
-  valid_result P f Q ∧ P s ⇒
+Theorem spec_total_imp:
+  spec_total P f Q ∧ P s ⇒
   ∃r t. f s = (INL r, t) ∧ Q r t
 Proof
-  rw[valid_result_def]
-  \\ drule valid_imp
+  rw[spec_total_def]
+  \\ drule spec_imp
   \\ disch_then drule
   \\ rw[] \\ gvs[]
   \\ Cases_on`r` \\ gvs[]
 QED
 
-Theorem valid_result_eq_imp:
-  valid_result_eq P f Q x ∧ P s ⇒
+Theorem spec_total_eq_imp:
+  spec_total_eq P f Q x ∧ P s ⇒
   ∃t. f s = (INL x, t) ∧ Q t
 Proof
-  rw[valid_result_eq_def, valid_result_fn_def]
-  \\ drule valid_result_imp
+  rw[spec_total_eq_def, spec_total_fn_def]
+  \\ drule spec_total_imp
   \\ disch_then drule
   \\ rw[]
 QED
